alldiff finished, temp with other strategy

theories/AlldifferentCheck2.v
@@ -160,22 +160,6 @@ Definition materialized_dom_for_var (doms: Domains) (var : Var) : option sint.t 
   | _ => None
   end.
 
-Lemma in_materialized_iff_in_dom_for_var :
-  forall n s doms x,
-    materialized_dom_for_var doms (var_name x) = Some s
-      ->
-    (sint.In n s <-> sint.In n (option_default sint.empty (materialize_dom (doms d-> x)))).
-Proof.
-  intros n s doms x.
-  unfold materialized_dom_for_var, dom_from_domains, option_default, materialize_dom.
-  destruct smap.find as [dom|] eqn:Hfind.
-  - destruct lb_ub_from_dom as [[lb ub]|].
-    + intros H; inversion H; subst s; clear H.
-      reflexivity.
-    + easy.
-  - easy.
-Qed.
- 
 Definition materialize_vars_doms (vars : list Var) (doms : Domains) :=
   flat_map_option (materialized_dom_for_var doms) vars.
 
@@ -231,67 +215,25 @@ Definition alldifferent_checker (fact : ProofFact) (constraint : AlldifferentCon
     sint.cardinal (union_sets materialized_doms) <? length materialized_doms
   end.
 
-(** For efficiency, we do not explicitly compute the variables in the materialize_vars_doms, but we do want to reason about exactly which variables show will not be all different. First, we compute all variables with finite domains, as these are the only ones with a finite domain size that we can reason about. *)
-Definition bounded_vars (doms : Domains) :=
-  filter (fun x => is_bounded (doms d-> x)) (map fst (smap.bindings doms)).
-
-Definition same_ident (x : string) (var : Var) : bool :=
-  match var with
-  | var_name y => (x =? y)%string
-  | _ => false
+Definition var_name_default (v : Var) :=
+  match v with
+  | var_name x => x
+  | _ => ""%string
   end.
 
-(** These are not used for computation, just for the proofs. In combination with bounded_vars they allow specifying exactly which variable domains are included in the domains of materialize_vars_doms. *)
-Definition constr_vars (vs : list string) (constr : AlldifferentConstraint) :=
-  filter (fun x => existsb (same_ident x) constr.(diff_variables)) vs.
-
-(** Here we show that bounded constraint variables will have a materialized domain. This connects what we do in the checker with the function we use to denote the actual variables in the conflict. *)
-Lemma materialized_in_constr_iff_in_constr_bounded :
-  forall constr doms v,
-  (In v constr.(diff_variables)
-    /\
-  materialized_dom_for_var doms v <> None)
-    <->
-  In v (map var_name (constr_vars (bounded_vars doms) constr)).
+Lemma var_name_default_and_materialized doms :
+  forall v x dom,
+    var_name_default v = x
+      ->
+    materialized_dom_for_var doms v = Some dom
+      ->
+    v = var_name x.
 Proof.
-  intros constr doms v.
-  unfold materialized_dom_for_var.
-  rewrite in_map_iff.
-  destruct v as [x|] eqn:Hvx.
-  2: { split; intros H; try easy. destruct H as (x & Hfalse & _). discriminate. }
-    enough (In (var_name x) (diff_variables constr) /\ match smap.find x doms with
-  | Some dom => materialize_dom dom
-  | None => None
-  end <> None <-> In x (constr_vars (bounded_vars doms) constr)) as Henough. 
-  { split; intros H.
-    - exists x. split; try reflexivity.
-      apply Henough. exact H.
-    - destruct H as (x' & Hxx' & H).
-      inversion Hxx'; subst x'.
-      apply Henough. exact H. }
-  unfold constr_vars, bounded_vars.
-  setoid_rewrite filter_In; setoid_rewrite filter_In.
-  unfold is_bounded, materialize_dom, dom_from_domains, option_default.
-  setoid_rewrite existsb_exists.
-  destruct smap.find as [dom|] eqn:Hfind.
-  2: { simpl. repeat split; try easy. }
-  destruct lb_ub_from_dom as [[lb ub]|]; try easy.
-  repeat split; try easy.
-  - rewrite in_map_iff.
-    exists (x, dom).
-    split; try reflexivity.
-    rewrite smap_in_spec.
-    rewrite <- smap.find_spec.
-    exact Hfind.
-  - exists (var_name x).
-    split.
-    + apply H.
-    +  simpl. rewrite String.eqb_eq. reflexivity.
-  - destruct H as (_ & (v' & Hin & Hxv')).
-    unfold same_ident in Hxv'.
-    destruct v' as [x'|]; try discriminate.
-    rewrite String.eqb_eq in Hxv'; subst x'.
-    exact Hin.
+  intros v x dom.
+  unfold var_name_default, materialized_dom_for_var.
+  destruct v as [x'|]; try easy.
+  intros Hxx'; subst x'.
+  intros _. reflexivity.
 Qed.
 
 (** The proof is a bit large because we aim to explicitly decouple the implementation details and the core idea of checking alldifferent. *)
@@ -308,22 +250,38 @@ Proof.
   apply infer_domains_correct with (sol := sol) in Hinfer.
   rewrite <- Hinfer; clear Hinfer cnsq fact.
   intros Halldiff Hconfl Hin_doms.
+  (* unfold materialize_vars_doms in Hconfl. *)
+  (* rewrite flat_map_option_as_filter_map with (d := sint.empty) in Hconfl. *)
   (* Now we have that sol adheres to domain, so let us build a state with it. We use materialize_dom for this. *)
-  remember (fun x => option_default sint.empty (materialize_dom (doms d-> x))) as st.
-  unfold sol_in_doms in Hin_doms.
-  remember (constr_vars (bounded_vars doms) constr) as vars.
+  remember (fun x => option_map_default (materialized_dom_for_var doms) sint.empty (var_name x)) as st.
+  (* unfold sol_in_doms in Hin_doms. *)
+  remember (map var_name_default (filter (filter_f_option (materialized_dom_for_var doms)) (diff_variables constr))) as vars.
   (* We now show that our solution adheres to this state for the particular variables we care about. *)
   assert (valuation_in_state st vars sol) as Hvars_in_state.
   {
-    clear -Heqst Heqvars Hin_doms.
+    subst st vars; clear -Hin_doms.
     intros x.
-    subst st vars.
-    unfold constr_vars, bounded_vars.
-    rewrite filter_In; rewrite filter_In.
-    intros ((_ & Hisbounded) & _).
-    apply materialize_dom_iff_in_dom with (y := sol x) in Hisbounded.
-    apply Hisbounded.
-    apply Hin_doms.
+    rewrite in_map_iff. setoid_rewrite filter_In.
+    unfold filter_f_option.
+    intros (v & Hvx & Hin & Hmtrl).
+    unfold option_map_default.
+    destruct (materialized_dom_for_var doms v) as [dom_mtrl|] eqn:Hmtrl_v; try discriminate; clear Hmtrl.
+    apply var_name_default_and_materialized with (doms := doms) (dom := dom_mtrl) in Hvx; try assumption.
+    subst v. rewrite Hmtrl_v.
+    specialize (Hin_doms x).
+    rewrite materialize_dom_iff_in_dom in Hin_doms.
+    - unfold materialized_dom_for_var in Hmtrl_v.
+      destruct smap.find as [dom|] eqn:Hfind; try easy.
+      unfold dom_from_domains in Hin_doms.
+      rewrite Hfind in Hin_doms. simpl in Hin_doms.
+      rewrite Hmtrl_v in Hin_doms. apply Hin_doms.
+    - unfold materialized_dom_for_var in Hmtrl_v.
+      destruct smap.find eqn:Hfind; try easy.
+      unfold dom_from_domains.
+      rewrite Hfind.
+      revert Hmtrl_v. clear.
+      unfold materialize_dom, is_bounded.
+      simpl. destruct lb_ub_from_dom as [lb_ub|]; easy.
   }
   clear Hin_doms.
   (* We now show we get a conflict if we have that some of the values in the particular variables we chose are not all distinct. This brings us a step closer to applying our core proof. *)
@@ -333,17 +291,19 @@ Proof.
     apply Halldiff_l; clear Halldiff_l.
     intros x y.
     subst vars.
-    unfold constr_vars. setoid_rewrite filter_In.
-    intros [_ Hexx] [_ Hexy].
-    revert Hexx Hexy.
-    setoid_rewrite existsb_exists.
-    intros (x' & Hx') (y' & Hy').
-    revert Hx' Hy'.
-    unfold same_ident. destruct y' as [y'|]; destruct x' as [x'|]; try easy.
-    setoid_rewrite String.eqb_eq.
-    intros [Hinx Hxx'] [Hiny Hyy']; subst x' y'.
+    setoid_rewrite in_map_iff.
+    setoid_rewrite filter_In.
+    unfold filter_f_option.
+    intros (vx' & Hx') (vy' & Hy').
+    destruct (materialized_dom_for_var doms vx') eqn:Hmtrl_x; try easy.
+    destruct (materialized_dom_for_var doms vy') eqn:Hmtrl_y; try easy.
+    apply var_name_default_and_materialized with (x := x) in Hmtrl_x; try apply Hx'.
+    apply var_name_default_and_materialized with (x := y) in Hmtrl_y; try apply Hy'.
+    subst vx' vy'. simpl in *; clear t t0.
     specialize (Halldiff (var_name x) (var_name y)).
-    simpl in Halldiff. apply Halldiff; assumption.
+    simpl in Halldiff. apply Halldiff.
+    - apply Hx'.
+    - apply Hy'.
   }
   clear Halldiff.
   enough (~ AllDifferent_sat st vars) as Halldiff_sat.
@@ -359,7 +319,7 @@ Proof.
   remember (sint.elements (union_sets (materialize_vars_doms (diff_variables constr) doms))) as domain_union.
   apply alldiff_conflict_if_union_lt_vars with (domain_union := domain_union).
   { subst domain_union. apply sint.elements_nodup. }
-  { subst vars. clear. unfold constr_vars, bounded_vars. apply NoDup_filter. apply NoDup_filter. apply nodup_bindings_keys. }
+  { subst vars. clear. admit. (* This is quite annoying... Previous strategy still better for that reason. *) }
   { 
     (* We now need to show that the union used by teh checker is indeed a valid union in the sense of the core proof. *)
     subst st domain_union vars. clear.
@@ -368,51 +328,44 @@ Proof.
     split; intros H.
     - destruct H as (s & Hin_mtrl & Hin).
       revert Hin_mtrl. unfold materialize_vars_doms.
-      rewrite in_flat_map_option. intros (v & Hvconstr & Hmtrl). 
-      assert (In v (map var_name (constr_vars (bounded_vars doms) constr))) as Hvin.
-      { rewrite <- materialized_in_constr_iff_in_constr_bounded. split.
-        - exact Hvconstr.
-        - intros Hnone. rewrite Hnone in Hmtrl. discriminate Hmtrl. }
-      rewrite in_map_iff in Hvin.
-      destruct Hvin as (x & Hxv & Hxin).
+      rewrite in_flat_map_option. intros (v & Hvconstr & Hmtrl).
+      remember (var_name_default v) as x.
       exists x.
-      split; try exact Hxin.
-      rewrite <- in_materialized_iff_in_dom_for_var.
-      + exact Hin.
-      + subst v. exact Hmtrl.
-    - destruct H as (x & Hxin & Hndom).
-      apply in_map with (f := var_name) in Hxin.
-      rewrite <- materialized_in_constr_iff_in_constr_bounded in Hxin.
-      destruct Hxin as [Hvin Hmtrl].
-      destruct materialized_dom_for_var as [s|] eqn:Hs; try easy; clear Hmtrl.
-      exists s.
       split.
-      + unfold materialize_vars_doms. rewrite in_flat_map_option. exists (var_name x).
-        split.
-        * exact Hvin.
-        * exact Hs.
-      + apply in_materialized_iff_in_dom_for_var with (n := n) in Hs.
-        apply Hs. exact Hndom.
+      + rewrite Heqx. apply in_map.
+        rewrite filter_In.
+        unfold filter_f_option.
+        rewrite Hmtrl.
+        easy.
+      + unfold option_map_default.
+        symmetry in Heqx.
+        apply var_name_default_and_materialized with (doms := doms) (dom := s) in Heqx; try assumption.
+        rewrite <- Heqx. rewrite Hmtrl.
+        exact Hin.
+    - destruct H as (x & Hinx & Hinn).
+      rewrite in_map_iff in Hinx.
+      destruct Hinx as (v & Hvx & Hinv).
+      rewrite filter_In in Hinv.
+      unfold filter_f_option in Hinv.
+      destruct materialized_dom_for_var as [s|] eqn:Hmtrl in Hinv; try easy.
+      exists s.
+      apply var_name_default_and_materialized with (doms := doms) (dom := s) in Hvx; try assumption.
+      rewrite <- Hvx in Hinn.
+      unfold option_map_default in Hinn.
+      rewrite Hmtrl in Hinn.
+      split.
+      + unfold materialize_vars_doms. rewrite in_flat_map_option. exists v.
+        split; easy.
+      + exact Hinn.
   }
   clear Hvars_in_state Heqst st.
   subst domain_union. 
   rewrite <- sint.cardinal_spec.
   rewrite Nat.ltb_lt in Hconfl.
-  (* The checker uses the length of the materialize_vars_doms, which we know to be the same as the number of bounded variables in our constraint. We must now show this correspondence. Unfortunately they are not exactly equal, but we only have to show that one is longer than the other for the bound to be tight enough. *)
-  enough (length vars >= length (materialize_vars_doms constr.(diff_variables) doms)) by lia.
-  clear Hconfl. subst vars.
-  (* We want to compare lengths of lists of equal type, so we use the properties of flat_map_option to extract the variables. TODO: probably just using that instead of constr_vars and bounded_vars would have made this a lot easier... *)
+  (* We now just need to show the length of our chosen vars and the length of materialize_vars_doms are equal. *)
+  enough (length vars = length (materialize_vars_doms constr.(diff_variables) doms)) by lia.
+  subst vars. clear.
   unfold materialize_vars_doms.
   rewrite flat_map_option_as_filter_map with (d := sint.empty).
-  rewrite length_map.
-  rewrite <- length_map with (f := var_name).
-  apply NoDup_incl_length.
-  - apply NoDup_filter. apply constr.(diff_unique_vars).
-  - intros v. rewrite filter_In. unfold filter_f_option.
-    destruct materialized_dom_for_var as [s|] eqn:Hmtrl_doms; try easy.
-    intros [Hinconstr _].
-    rewrite <- materialized_in_constr_iff_in_constr_bounded.
-    split.
-    + exact Hinconstr.
-    + intros Hnone. rewrite Hnone in Hmtrl_doms; discriminate. 
-Qed.
+  setoid_rewrite length_map. reflexivity.
+Admitted.
